Will need boostrapping

src/Init/Data/UInt/Basic.lean
@@ -9,6 +9,10 @@ import Init.Data.BitVec.Basic
 
 open Nat
 
+@[inline, deprecated ofNatLT (since := "2025-02-12"), inherit_doc ofNatLT]
+def UInt8.ofNatCore (n : Nat) (h : n < UInt8.size) : UInt8 :=
+  UInt8.ofNatLT n h
+
 @[extern "lean_uint8_add"]
 def UInt8.add (a b : UInt8) : UInt8 := ⟨a.toBitVec + b.toBitVec⟩
 @[extern "lean_uint8_sub"]
@@ -71,6 +75,10 @@ instance (a b : UInt8) : Decidable (a < b) := UInt8.decLt a b
 instance (a b : UInt8) : Decidable (a ≤ b) := UInt8.decLe a b
 instance : Max UInt8 := maxOfLe
 instance : Min UInt8 := minOfLe
+
+@[inline, deprecated ofNatLT (since := "2025-02-12"), inherit_doc ofNatLT]
+def UInt16.ofNatCore (n : Nat) (h : n < UInt16.size) : UInt16 :=
+  UInt16.ofNatLT n h
 
 @[extern "lean_uint16_add"]
 def UInt16.add (a b : UInt16) : UInt16 := ⟨a.toBitVec + b.toBitVec⟩
@@ -137,6 +145,10 @@ instance (a b : UInt16) : Decidable (a ≤ b) := UInt16.decLe a b
 instance : Max UInt16 := maxOfLe
 instance : Min UInt16 := minOfLe
 
+@[inline, deprecated ofNatLT (since := "2025-02-12"), inherit_doc ofNatLT]
+def UInt32.ofNatCore (n : Nat) (h : n < UInt32.size) : UInt32 :=
+  UInt32.ofNatLT n h
+
 @[extern "lean_uint32_add"]
 def UInt32.add (a b : UInt32) : UInt32 := ⟨a.toBitVec + b.toBitVec⟩
 @[extern "lean_uint32_sub"]
@@ -186,6 +198,10 @@ instance : ShiftRight UInt32 := ⟨UInt32.shiftRight⟩
 
 @[extern "lean_bool_to_uint32"]
 def Bool.toUInt32 (b : Bool) : UInt32 := if b then 1 else 0
+
+@[inline, deprecated ofNatLT (since := "2025-02-12"), inherit_doc ofNatLT]
+def UInt64.ofNatCore (n : Nat) (h : n < UInt64.size) : UInt64 :=
+  UInt64.ofNatLT n h
 
 @[extern "lean_uint64_add"]
 def UInt64.add (a b : UInt64) : UInt64 := ⟨a.toBitVec + b.toBitVec⟩
@@ -250,6 +266,10 @@ instance (a b : UInt64) : Decidable (a ≤ b) := UInt64.decLe a b
 instance : Max UInt64 := maxOfLe
 instance : Min UInt64 := minOfLe
 
+@[inline, deprecated ofNatLT (since := "2025-02-12"), inherit_doc ofNatLT]
+def USize.ofNatCore (n : Nat) (h : n < USize.size) : USize :=
+  USize.ofNatLT n h
+
 theorem usize_size_le : USize.size ≤ 18446744073709551616 := by
   cases usize_size_eq <;> next h => rw [h]; decide
 
@@ -281,7 +301,7 @@ This function is overridden with a native implementation.
 -/
 @[extern "lean_usize_of_nat"]
 def USize.ofNat32 (n : @& Nat) (h : n < 4294967296) : USize :=
-  USize.ofNatCore n (Nat.lt_of_lt_of_le h le_usize_size)
+  USize.ofNatLT n (Nat.lt_of_lt_of_le h le_usize_size)
 @[extern "lean_uint8_to_usize"]
 def UInt8.toUSize (a : UInt8) : USize :=
   USize.ofNat32 a.toBitVec.toNat (Nat.lt_trans a.toBitVec.isLt (by decide))
@@ -306,7 +326,7 @@ This function is overridden with a native implementation.
 -/
 @[extern "lean_usize_to_uint64"]
 def USize.toUInt64 (a : USize) : UInt64 :=
-  UInt64.ofNatCore a.toBitVec.toNat (Nat.lt_of_lt_of_le a.toBitVec.isLt usize_size_le)
+  UInt64.ofNatLT a.toBitVec.toNat (Nat.lt_of_lt_of_le a.toBitVec.isLt usize_size_le)
 
 instance : Mul USize       := ⟨USize.mul⟩
 instance : Mod USize       := ⟨USize.mod⟩
